Simplify

Abstract_Formula.thy
@@ -5,6 +5,14 @@ imports
   "~~/src/HOL/Library/Stream"
 begin
 
+context includes fset.lifting
+begin
+lift_definition fset_from_list :: "'a list => 'a fset" is set by (rule finite_set)
+lemma mem_fset_from_list[simp]: "x |\<in>| fset_from_list l  \<longleftrightarrow> x \<in> set l" by transfer rule
+lemma fimage_fset_from_list[simp]: "f |`| fset_from_list l = fset_from_list (map f l)"  by transfer auto
+end
+
+
 locale Abstract_Formulas =
   fixes annotate :: "'annot \<Rightarrow> 'preform \<Rightarrow> 'form"
   fixes pre_fv :: "'preform \<Rightarrow> 'var set"
@@ -20,6 +28,12 @@ locale Abstract_Rules =
   fixes antecedent :: "'rule \<Rightarrow> ('preform list \<times> 'preform) list"
   fixes consequent :: "'rule \<Rightarrow> 'preform list"
   and rules :: "'rule stream"
+begin
+  definition f_antecedent :: "'rule \<Rightarrow> ('preform fset \<times> 'preform) fset"
+    where "f_antecedent r = (fset_from_list (map (apfst fset_from_list) (antecedent r)))"
+  definition "f_consequent r = (fset_from_list (consequent r))"
+
+end
 
 locale Abstract_Task =
   Abstract_Rules  _ _ _ pre_fv _ _ _ rules
@@ -27,13 +41,6 @@ locale Abstract_Task =
   fixes assumptions :: "'preform list"
   fixes conclusions :: "'preform list"
   assumes no_empty_conclusions: "\<forall>xs\<in>sset rules. consequent xs \<noteq> []"
-
-context includes fset.lifting
-begin
-lift_definition fset_from_list :: "'a list => 'a fset" is set by (rule finite_set)
-lemma mem_fset_from_list[simp]: "x |\<in>| fset_from_list l  \<longleftrightarrow> x \<in> set l" by transfer rule
-lemma fimage_fset_from_list[simp]: "f |`| fset_from_list l = fset_from_list (map f l)"  by transfer auto
-end
 
 
 end
